driver/Compiler.v
@@ -350,9 +350,10 @@ Qed.
 
 Section WITHEXTERNALCALLS.
 Local Existing Instance Events.symbols_inject_instance.
-Context `{external_calls_prf: Events.ExternalCalls (symbols_inject'_instance := Events.symbols_inject_instance) }.
+Context `{external_calls_prf: Events.ExternalCalls (symbols_inject_instance := Events.symbols_inject_instance) }.
 Context {i64_helpers_correct_prf: SelectLongproof.I64HelpersCorrect mem}.
 Context `{memory_model_x_prf: !Unusedglobproof.Mem.MemoryModelX mem}.
+
 
 Theorem cstrategy_semantic_preservation:
   forall p tp,
@@ -392,7 +393,7 @@ Ltac DestructM :=
   eapply compose_forward_simulations.
     eapply match_if_simulation. eassumption. exact Renumberproof.transf_program_correct.
   eapply compose_forward_simulations.
-    eapply match_if_simulation. eassumption. exact CSEproof.transf_program_correct.
+    eapply match_if_simulation. eassumption. eapply CSEproof.transf_program_correct; assumption.
   eapply compose_forward_simulations.
     eapply match_if_simulation. eassumption. exact Deadcodeproof.transf_program_correct; eassumption.
   eapply compose_forward_simulations.
@@ -408,7 +409,7 @@ Ltac DestructM :=
   eapply compose_forward_simulations.
     eapply match_if_simulation. eassumption. exact Debugvarproof.transf_program_correct.
   eapply compose_forward_simulations.
-    eapply Stackingproof.transf_program_correct with (return_address_offset := Asmgenproof0.return_address_offset).
+    eapply Stackingproof.transf_program_correct with (return_address_offset := Asmgenproof0.return_address_offset); try assumption.
     exact Asmgenproof.return_address_exists.
     eassumption.
   eapply Asmgenproof.transf_program_correct; eassumption.
